pulse/examples/dsls/mini_steel/Pulse.Checker.Common.fsti
@@ -7,7 +7,14 @@ open FStar.List.Tot
 open Pulse.Syntax
 open Pulse.Elaborate.Pure
 open Pulse.Typing
-  
+
+val force_st (#f:_) (#g:_) (#t:_) (#pre:pure_term)
+  (pre_typing:tot_typing f g pre Tm_VProp)
+  (x:(c:pure_comp { stateful_comp c ==> comp_pre c == pre } & 
+      src_typing f g t c))
+  : T.Tac (c:pure_comp_st { comp_pre c == pre } &
+           src_typing f g t c)
+
 type check_t =
   f:RT.fstar_top_env ->
   g:env ->
